Moved variable, expanded Types slightly in prep for type checking

02Typed/Type.thy
@@ -1,7 +1,23 @@
 theory Type
-  imports Main
+  imports "../00Utils/Variable"
 begin
 
-datatype ty = Base | Arrow ty ty
+datatype ty = 
+  TVar var
+  | Base 
+  | Arrow ty ty
+
+primrec tsubst_var :: "var \<Rightarrow> var \<Rightarrow> ty \<Rightarrow> ty" where
+  "tsubst_var x x' (TVar y) = TVar (if x = y then x' else y)"
+| "tsubst_var x x' Base = Base"
+| "tsubst_var x x' (Arrow t\<^sub>1 t\<^sub>2) = Arrow (tsubst_var x x' t\<^sub>1) (tsubst_var x x' t\<^sub>2)"
+
+lemma [simp]: "size (tsubst_var x x' t) = size t"
+  by (induction t) simp_all
+
+fun tsubst :: "var \<Rightarrow> ty \<Rightarrow> ty \<Rightarrow> ty" where
+  "tsubst x t' (TVar y) = (if x = y then t' else TVar y)"
+| "tsubst x t' Base = Base"
+| "tsubst x t' (Arrow t\<^sub>1 t\<^sub>2) = Arrow (tsubst x t' t\<^sub>1) (tsubst x t' t\<^sub>2)"
 
 end
